src/3d/CoerceProbes.fst
@@ -26,6 +26,7 @@ open FStar.All
 module H = Hashtable
 module B = Binding
 open GlobalEnv
+open GeneralizeProbes
 
 let probe_fail
 : probe_action
@@ -38,31 +39,6 @@ let probe_return_unit
 = with_dummy_range <|
   Probe_atomic_action <|
   Probe_action_return (with_dummy_range (Constant Unit))
-
-let print_probe_qualifier = function
-  | PQWithOffsets -> "WithOffsets"
-  | PQRead i -> Printf.sprintf "Read %s" (print_integer_type i)
-  | PQWrite i -> Printf.sprintf "Write %s" (print_integer_type i)
-  | PQInit -> "Init"
-
-
-let find_probe_fn (e:B.env) (q:probe_qualifier)
-: ML ident
-= match GlobalEnv.extern_probe_fn_qual (B.global_env_of_env e) (Some q) with
-  | None ->
-    error (Printf.sprintf "Cannot find probe function for %s" (print_probe_qualifier q))
-          dummy_range
-  | Some id ->
-    id
-  
-let find_extern_coercion (e:B.env) (t0:typ) (t1:typ)
-: ML ident
-= match GlobalEnv.resolve_extern_coercion (B.global_env_of_env e) t0 t1 with
-  | None ->
-    error (Printf.sprintf "Cannot find coercion for %s to %s" (print_typ t0) (print_typ t1))
-          dummy_range
-  | Some id ->
-    id
 
 let read_and_coerce_pointer (e:B.env) (fid:ident) (k:probe_action)
 : ML probe_action
