src/3d/prelude/EverParse3d.Actions.Base.fsti
@@ -911,6 +911,7 @@ inline_for_extraction
 noextract
 val probe_then_validate
       (#nz:bool)
+      (#maybe_zero_offset:bool)
       (#wk: _)
       (#k:parser_kind nz wk)
       (#t:Type)
@@ -929,7 +930,7 @@ val probe_then_validate
       (dest:CP.copy_buffer_t)
       (init:PA.init_probe_dest_t)
       (prep_dest_sz:U64.t)
-      (probe:PA.probe_m unit true)
+      (probe:PA.probe_m unit true maybe_zero_offset)
   : action (conj_inv inv (copy_buffer_inv dest))
            (conj_disjointness disj (disjoint (copy_buffer_loc dest) l))
            (eloc_union l (copy_buffer_loc dest)) 
